@prefix smurf: <http://geosensor.net/SMURF#> .
@prefix dqv: <http://www.w3.org/ns/dqv#> .
@prefix geo: <http://www.opengis.net/ont/geosparql#> .
@prefix owl: <http://www.w3.org/2002/07/owl#> .
@prefix rdf: <http://www.w3.org/1999/02/22-rdf-syntax-ns#> .
@prefix xml: <http://www.w3.org/XML/1998/namespace> .
@prefix xsd: <http://www.w3.org/2001/XMLSchema#> .
@prefix dcat: <http://www.w3.org/ns/dcat#> .
@prefix rdfs: <http://www.w3.org/2000/01/rdf-schema#> .
@base <http://geosensor.net/SMURF> .

<http://geosensor.net/SMURF> rdf:type owl:Ontology .

#################################################################
#    Annotation properties
#################################################################

###  http://www.w3.org/2004/02/skos/core#definition
<http://www.w3.org/2004/02/skos/core#definition> rdf:type owl:AnnotationProperty .


###  http://www.w3.org/2004/02/skos/core#example
<http://www.w3.org/2004/02/skos/core#example> rdf:type owl:AnnotationProperty .


#################################################################
#    Datatypes
#################################################################

###  http://www.opengis.net/ont/geosparql#wktLiteral
geo:wktLiteral rdf:type rdfs:Datatype .


###  http://www.w3.org/2001/XMLSchema#date
xsd:date rdf:type rdfs:Datatype .


#################################################################
#    Object Properties
#################################################################

###  http://geosensor.net/SMURF#hasGeometryProvenance
:hasGeometryProvenance rdf:type owl:ObjectProperty ;
                       rdfs:domain geo:Geometry ;
                       rdfs:range dcat:Dataset ;
                       rdfs:comment "hasGeometryProvenance indicates the provenance (i.e., source, quality, and other metadata) of a GeoSPAQL Geometry in terms of a DCAT Dataset instance."@en ;
                       rdfs:label "hasGeometryProvenance"@en ;
                       <http://www.w3.org/2004/02/skos/core#definition> "hasGeometryProvenance indicates the provenance (i.e., source, quality, and other metadata) of a GeoSPAQL Geometry in terms of a DCAT Dataset instance."@en ;
                       <http://www.w3.org/2004/02/skos/core#example> "Geometry x is from (hahsGeometryProvenance) Dataset y"@en .


#################################################################
#    Data properties
#################################################################

###  http://geosensor.net/SMURF#createDate
:createDate rdf:type owl:DatatypeProperty ;
            rdfs:domain geo:Geometry ;
            rdfs:range xsd:date ;
            rdfs:comment "The date on which this Geometry was created"@en ;
            rdfs:label "Creation date"@en ;
            <http://www.w3.org/2004/02/skos/core#definition> "The date on which this Geometry was created"@en .


###  http://geosensor.net/SMURF#geometryCoordinates
:geometryCoordinates rdf:type owl:DatatypeProperty ;
                     rdfs:subPropertyOf geo:asWKT ;
                     rdfs:domain geo:Geometry ;
                     rdfs:range geo:wktLiteral ;
                     rdfs:comment "WKT geometry coordinates for a Geometry instance"@en ;
                     rdfs:label "Geometry coordinates"@en ;
                     <http://www.w3.org/2004/02/skos/core#definition> "WKT geometry coordinates for a Geometry instance"@en .


###  http://geosensor.net/SMURF#hasPFI
:hasPFI rdf:type owl:DatatypeProperty ;
        rdfs:domain geo:Geometry ;
        rdfs:range xsd:integer ;
        rdfs:comment "Indicates the VicMap PFI (persistent feature identifier) for this Geometry"@en ;
        rdfs:label "Has PFI (persistent feature identifier)"@en ;
        <http://www.w3.org/2004/02/skos/core#definition> "Indicates the VicMap PFI (persistent feature identifier) for this Geometry"@en .


###  http://geosensor.net/SMURF#hasUFI
:hasUFI rdf:type owl:DatatypeProperty ;
        rdfs:domain geo:Geometry ;
        rdfs:range xsd:integer ;
        rdfs:comment "Indicates the VicMap UFI (unique feature identifier) for this Geometry"@en ;
        rdfs:label "Has UFI (unique feature identifier)"@en ;
        <http://www.w3.org/2004/02/skos/core#definition> "Indicates the VicMap UFI (unique feature identifier) for this Geometry"@en .


###  http://geosensor.net/SMURF#isAuthoritativeData
:isAuthoritativeData rdf:type owl:DatatypeProperty ;
                     rdfs:domain dqv:QualityMeasurement ;
                     rdfs:range xsd:boolean ;
                     rdfs:comment "Flag to indicate if this data item is an authoritative VicMap version (true) or not (false)"@en ;
                     rdfs:label "Is authoritative data version"@en ;
                     <http://www.w3.org/2004/02/skos/core#definition> "Flag to indicate if this data item is an authoritative VicMap version (true) or not (false)"@en .


###  http://geosensor.net/SMURF#isCrown
:isCrown rdf:type owl:DatatypeProperty ;
         rdfs:domain geo:Geometry ;
         rdfs:range xsd:boolean ;
         rdfs:comment "Flag to indicate if this data item is a Crown land (true) or not (false)"@en ;
         rdfs:label "Is Crown"@en ;
         <http://www.w3.org/2004/02/skos/core#definition> "Flag to indicate if this data item is a Crown land (true) or not (false)"@en .


###  http://geosensor.net/SMURF#organizationemail
:organizationemail rdf:type owl:DatatypeProperty ;
                   rdfs:domain <http://www.w3.org/ns/prov#Organization> ;
                   rdfs:range xsd:string ;
                   rdfs:comment "Organization email address"@en ;
                   rdfs:label "Organization email"@en ;
                   <http://www.w3.org/2004/02/skos/core#definition> "Organization email address"@en .


###  http://geosensor.net/SMURF#personalemail
:personalemail rdf:type owl:DatatypeProperty ;
               rdfs:domain <http://www.w3.org/ns/prov#Person> ;
               rdfs:range xsd:string ;
               rdfs:comment "Personal email address"@en ;
               rdfs:label "Personal email"@en ;
               <http://www.w3.org/2004/02/skos/core#definition> "Personal email address"@en .


###  http://geosensor.net/SMURF#varietyOf
:varietyOf rdf:type owl:DatatypeProperty ;
           rdfs:domain geo:Geometry ;
           rdfs:range xsd:string ;
           rdfs:comment "Water body type attribute, indicating the type of hydrology feature"@en ;
           rdfs:label "Variety of"@en ;
           <http://www.w3.org/2004/02/skos/core#definition> "Water body type attribute, indicating the type of hydrology feature"@en ;
           <http://www.w3.org/2004/02/skos/core#example> "flat_sti"@en ,
                                                         "wb_dam"@en ,
                                                         "wb_lake"@en .


###  http://geosensor.net/SMURF#waterbodyID
:waterbodyID rdf:type owl:DatatypeProperty ;
             rdfs:domain geo:Feature ;
             rdfs:range xsd:integer ;
             rdfs:comment "Vicmap waterbody idenfitier"@en ;
             rdfs:label "Waterbody ID"@en ;
             <http://www.w3.org/2004/02/skos/core#example> "Vicmap waterbody idenfitier"@en .


###  http://www.opengis.net/ont/geosparql#asWKT
geo:asWKT rdf:type owl:DatatypeProperty .


#################################################################
#    Classes
#################################################################

###  http://www.opengis.net/ont/geosparql#Feature
geo:Feature rdf:type owl:Class .


###  http://www.opengis.net/ont/geosparql#Geometry
geo:Geometry rdf:type owl:Class .


###  http://www.w3.org/ns/dcat#Dataset
dcat:Dataset rdf:type owl:Class .


###  http://www.w3.org/ns/dqv#QualityMeasurement
dqv:QualityMeasurement rdf:type owl:Class .


###  http://www.w3.org/ns/prov#Organization
<http://www.w3.org/ns/prov#Organization> rdf:type owl:Class .


###  http://www.w3.org/ns/prov#Person
<http://www.w3.org/ns/prov#Person> rdf:type owl:Class .


###  Generated by the OWL API (version 4.5.9.2019-02-01T07:24:44Z) https://github.com/owlcs/owlapi
