@prefix : <http://geosensor.net/ns/SMURF#> .
@prefix owl: <http://www.w3.org/2002/07/owl#> .
@prefix rdf: <http://www.w3.org/1999/02/22-rdf-syntax-ns#> .
@prefix xml: <http://www.w3.org/XML/1998/namespace> .
@prefix xsd: <http://www.w3.org/2001/XMLSchema#> .
@prefix rdfs: <http://www.w3.org/2000/01/rdf-schema#> .
@base <http://geosensor.net/ns/SMURF> .

<http://geosensor.net/ns/SMURF> rdf:type owl:Ontology ;
                                 owl:versionIRI <http://geosensor.net/ns/SMURF-250115> ;
                                 owl:imports <http://www.opengis.net/ont/geosparql> ,
                                             <http://www.w3.org/ns/dcat3> ,
                                             <http://www.w3.org/ns/dqv> ,
                                             <http://www.w3.org/ns/prov-o-20130430> .

#################################################################
#    Object Properties
#################################################################

###  http://geosensor.net/ns/SMURF#hasGeometryProvenance
:hasGeometryProvenance rdf:type owl:ObjectProperty ;
                       rdfs:subPropertyOf <http://www.w3.org/ns/prov#wasInfluencedBy> ;
                       rdfs:domain <http://www.opengis.net/ont/geosparql#Geometry> ;
                       rdfs:range <http://purl.org/linked-data/cube#DataSet> ;
                       rdfs:comment "hasGeometryProvenance indicates the provenance (i.e., source, quality, and other metadata) of a GeoSPARQL Geometry in terms of a DCAT Dataset instance."@en ;
                       rdfs:label "hasGeometryProvenance"@en ;
                       <http://www.w3.org/2004/02/skos/core#definition> "hasGeometryProvenance indicates the provenance (i.e., source, quality, and other metadata) of a GeoSPARQL Geometry in terms of a DCAT Dataset instance."@en ;
                       <http://www.w3.org/2004/02/skos/core#example> "Geometry x is from (hasGeometryProvenance) Dataset y"@en .


#################################################################
#    Data properties
#################################################################

###  http://geosensor.net/ns/SMURF#createDate
:createDate rdf:type owl:DatatypeProperty ;
            rdfs:domain <http://www.opengis.net/ont/geosparql#Geometry> ;
            rdfs:range xsd:date ;
            rdfs:comment "The date on which this Geometry was created"@en ;
            rdfs:label "Creation date"@en ;
            <http://www.w3.org/2004/02/skos/core#definition> "The date on which this Geometry was created"@en .


###  http://geosensor.net/ns/SMURF#geometryCoordinates
:geometryCoordinates rdf:type owl:DatatypeProperty ;
                     rdfs:subPropertyOf <http://www.opengis.net/ont/geosparql#asWKT> ;
                     rdfs:domain <http://www.opengis.net/ont/geosparql#Geometry> ;
                     rdfs:range <http://www.opengis.net/ont/geosparql#wktLiteral> ;
                     rdfs:comment "WKT geometry coordinates for a Geometry instance"@en ;
                     rdfs:label "Geometry coordinates"@en ;
                     <http://www.w3.org/2004/02/skos/core#definition> "WKT geometry coordinates for a Geometry instance"@en .


###  http://geosensor.net/ns/SMURF#hasPFI
:hasPFI rdf:type owl:DatatypeProperty ;
        rdfs:domain <http://www.opengis.net/ont/geosparql#Geometry> ;
        rdfs:range xsd:integer ;
        rdfs:comment "Indicates the VicMap PFI (persistent feature identifier) for this Geometry"@en ;
        rdfs:label "Has PFI (persistent feature identifier)"@en ;
        <http://www.w3.org/2004/02/skos/core#definition> "Indicates the VicMap PFI (persistent feature identifier) for this Geometry"@en .


###  http://geosensor.net/ns/SMURF#hasUFI
:hasUFI rdf:type owl:DatatypeProperty ;
        rdfs:domain <http://www.opengis.net/ont/geosparql#Geometry> ;
        rdfs:range xsd:integer ;
        rdfs:comment "Indicates the VicMap UFI (unique feature identifier) for this Geometry"@en ;
        rdfs:label "Has UFI (unique feature identifier)"@en ;
        <http://www.w3.org/2004/02/skos/core#definition> "Indicates the VicMap UFI (unique feature identifier) for this Geometry"@en .


###  http://geosensor.net/ns/SMURF#isAuthoritativeData
:isAuthoritativeData rdf:type owl:DatatypeProperty ;
                     rdfs:domain <http://www.w3.org/ns/dqv#QualityMeasurement> ;
                     rdfs:range xsd:boolean ;
                     rdfs:comment "Flag to indicate if this data item is an authoritative VicMap version (true) or not (false)"@en ;
                     rdfs:label "Is authoritative data version"@en ;
                     <http://www.w3.org/2004/02/skos/core#definition> "Flag to indicate if this data item is an authoritative VicMap version (true) or not (false)"@en .


###  http://geosensor.net/ns/SMURF#isCrown
:isCrown rdf:type owl:DatatypeProperty ;
         rdfs:domain <http://www.opengis.net/ont/geosparql#Geometry> ;
         rdfs:range xsd:boolean ;
         rdfs:comment "Flag to indicate if this data item is a Crown land (true) or not (false)"@en ;
         rdfs:label "Is Crown"@en ;
         <http://www.w3.org/2004/02/skos/core#definition> "Flag to indicate if this data item is a Crown land (true) or not (false)"@en .


###  http://geosensor.net/ns/SMURF#organizationEmail
:organizationEmail rdf:type owl:DatatypeProperty ;
                   rdfs:domain <http://www.w3.org/ns/prov#Organization> ;
                   rdfs:range xsd:string ;
                   rdfs:label "Organization email"@en ,
                              "Organization email address"@en ;
                   <http://www.w3.org/2004/02/skos/core#definition> "Organization email address"@en .


###  http://geosensor.net/ns/SMURF#personalEmail
:personalEmail rdf:type owl:DatatypeProperty ;
               rdfs:domain <http://www.w3.org/ns/prov#Person> ;
               rdfs:range xsd:string ;
               rdfs:comment "Personal email address"@en ;
               rdfs:label "Personal email"@en ;
               <http://www.w3.org/2004/02/skos/core#definition> "Personal email address"@en .


###  http://geosensor.net/ns/SMURF#varietyOf
:varietyOf rdf:type owl:DatatypeProperty ;
           rdfs:domain <http://www.opengis.net/ont/geosparql#Geometry> ;
           rdfs:range xsd:string ;
           rdfs:comment "Water body type attribute, indicating the type of hydrology feature"@en ;
           rdfs:label "Variety of"@en ;
           <http://www.w3.org/2004/02/skos/core#definition> "Water body type attribute, indicating the type of hydrology feature"@en .


###  http://geosensor.net/ns/SMURF#waterbodyID
:waterbodyID rdf:type owl:DatatypeProperty ;
             rdfs:domain <http://www.opengis.net/ont/geosparql#Feature> ;
             rdfs:range xsd:integer ;
             rdfs:comment "Vicmap waterbody identifier"@en ;
             rdfs:label "Waterbody ID"@en ;
             <http://www.w3.org/2004/02/skos/core#definition> "Vicmap waterbody identifier"@en .


###  Generated by the OWL API (version 4.5.29.2024-05-13T12:11:03Z) https://github.com/owlcs/owlapi
